seiostar/LogRelTargetSource.fst
@@ -17,7 +17,7 @@ let rec (∋) (t:qType) (p:(history * fs_val t * closed_exp)) : Tot Type0 (decre
   let (h, fs_v, e) = p in
   match get_rel t with // way to "match" on F* types
   | QUnit -> fs_v == () /\ e == EUnit
-  | QBool -> (fs_v == true /\ e == ETrue) \/ (fs_v == false /\ e == EFalse)
+  | QBool #ref -> (ref true /\ fs_v == true /\ e == ETrue) \/ (fs_v == false /\ e == EFalse)
   | QFileDescriptor ->  e == EFileDescr fs_v
   | QString -> (match e with | EString s -> fs_v == s | _ -> False)
   | QArr #t1 #t2 qt1 qt2 -> begin
@@ -28,8 +28,9 @@ let rec (∋) (t:qType) (p:(history * fs_val t * closed_exp)) : Tot Type0 (decre
         pack qt2 ⊇ (h++lt_v, fs_f fs_v, subst_beta v e'))
     | _ -> False
   end
-  | QArrIO #t1 #t2 qt1 qt2 -> begin
-    let fs_f : t1 -> io t2 = fs_v in
+  | QArrIO #t1 #t2 qt1 qt2 #post -> begin
+    let fs_f : (x:t1) -> io (y:t2{post x y}) = fs_v in
+    let fs_f : t1 -> io t2 = fun (x:t1) -> io_map (forget_ref #t1 #t2 #post x) (fs_f x) in
     match e with
     | ELam e' -> // instead quantify over h'' - extensions of the history
       (forall (v:value) (fs_v:t1) (lt_v:local_trace h). pack qt1 ∋ (h++lt_v, fs_v, v) ==>
@@ -49,7 +50,7 @@ let rec (∋) (t:qType) (p:(history * fs_val t * closed_exp)) : Tot Type0 (decre
     | Inr fs_v', EInr e' -> pack qt2 ∋ (h, fs_v', e')
     | _ -> False
   end
-  | QRefinement #t qt ref -> False // TODO
+  //| QRefinement #t qt ref -> False // TODO
 
                            (** vvvvvvvvvv defined over values **)
 and (⊇) (t:qType) (p:history * fs_val t * closed_exp) : Tot Type0 (decreases %[get_rel t;1]) =
@@ -173,23 +174,23 @@ let (∽) (#g:typ_env) #b (h:history) (fsG:eval_env g) (s:gsub g b) : Type0 =
 
 (** Cross Language Binary Logical Relation between F* and LambdaIO expressions
      for __open terms__. **)
-let superset_oval (#g:typ_env) (t:qType) (fs_e:fs_oval g t) (e:exp) : Type0 =
+let superset_oval (#g:typ_env) (t:qType) (#pre:spec_env g) (fs_e:fs_oval g t pre) (e:exp) : Type0 =
   fv_in_env g e /\
   forall b (s:gsub g b) (fsG:eval_env g) (h:history).
-    fsG `(∽) h` s ==> t ⊇ (h, fs_e fsG, gsubst s e)
+    (fsG `(∽) h` s /\ pre fsG) ==> t ⊇ (h, fs_e fsG, gsubst s e)
 
-let (⊐) (#g:typ_env) (#t:qType) (fs_v:fs_oval g t) (e:exp) : Type0 =
+let (⊐) (#g:typ_env) (#t:qType) (#pre:spec_env g) (fs_v:fs_oval g t pre) (e:exp) : Type0 =
   superset_oval #g t fs_v e
 
-let superset_ocomp (#g:typ_env) (t:qType) (fs_e:fs_ocomp g t) (e:exp) : Type0 =
+let superset_ocomp (#g:typ_env) (t:qType) (#pre:spec_env g) (fs_e:fs_ocomp g t pre) (e:exp) : Type0 =
   fv_in_env g e /\
   forall b (s:gsub g b) (fsG:eval_env g) (h:history).
-    fsG `(∽) h` s ==> t ⫄ (h, fs_e fsG, gsubst s e)
+    (fsG `(∽) h` s /\ pre fsG) ==> t ⫄ (h, fs_e fsG, gsubst s e)
 
-let (⊒) (#g:typ_env) (#t:qType) (fs_v:fs_ocomp g t) (e:exp) : Type0 =
+let (⊒) (#g:typ_env) (#t:qType) (#pre:spec_env g) (fs_v:fs_ocomp g t pre) (e:exp) : Type0 =
   superset_ocomp #g t fs_v e
 
-let lem_value_superset_valid_contains t (fs_e:fs_oval empty t) (e:value) :
+let lem_value_superset_valid_contains t (fs_e:fs_oval empty t (fun _ -> True)) (e:value) :
   Lemma (requires fs_e ⊐ e)
         (ensures  valid_contains #t (fs_e empty_eval) e) =
   introduce forall h. t ∋ (h, fs_e empty_eval, e) with begin
@@ -200,12 +201,12 @@ let lem_value_superset_valid_contains t (fs_e:fs_oval empty t) (e:value) :
     assert (t ∋ (h, fs_e empty_eval, e))
   end
 
-let lem_closed_superset_valid_prod g (fsG:eval_env g) #t #b (s:gsub g b) (fs_e:fs_ocomp g t) (e:exp) :
-  Lemma (requires fs_e ⊒ e /\ (forall h. fsG `(∽) h` s))
+let lem_closed_superset_valid_prod g (fsG:eval_env g) #t #b #pre (s:gsub g b) (fs_e:fs_ocomp g t pre) (e:exp) :
+  Lemma (requires fs_e ⊒ e /\ (forall h. fsG `(∽) h` s) /\ pre fsG)
         (ensures  valid_superset_comp #t (fs_e fsG) (gsubst s e)) =
   introduce forall h. t ⫄ (h, fs_e fsG, gsubst s e) with begin
     eliminate forall b (s:gsub g b) (fsG:eval_env g) (h:history).
-      fsG `(∽) h` s ==> t ⫄ (h, fs_e fsG, gsubst s e) with b s fsG h
+      (fsG `(∽) h` s /\ pre fsG) ==> t ⫄ (h, fs_e fsG, gsubst s e) with b s fsG h
   end
 
 let rec val_type_closed_under_history_extension (t:qType) (h:history) (fs_v:fs_val t) (e:closed_exp) :
@@ -228,8 +229,9 @@ let rec val_type_closed_under_history_extension (t:qType) (h:history) (fs_v:fs_v
       end
     end
     end
-  | QArrIO #t1 #t2 qt1 qt2 -> begin
-    let fs_f : t1 -> io t2 = fs_v in
+  | QArrIO #t1 #t2 qt1 qt2 #post -> begin
+    let fs_f : (x:t1) -> io (y:t2{post x y}) = fs_v in
+    let fs_f : t1 -> io t2 = fun (x:t1) -> io_map (forget_ref #t1 #t2 #post x) (fs_f x) in
     let ELam e' = e in
     introduce forall (v:value) (fs_v':t1) (lt_v':local_trace (h++lt)). pack qt1 ∋ ((h++lt)++lt_v', fs_v', v) ==> pack qt2 ⫄ ((h++lt)++lt_v', fs_f fs_v', subst_beta v e') with begin
       introduce pack qt1 ∋ ((h++lt)++lt_v', fs_v', v) ==> _ with _. begin
@@ -327,7 +329,7 @@ let unfold_contains_arrow (t1 t2:qType) (h:history) (fs_e1:fs_val (t1 ^-> t2)) (
   : Lemma
     (requires is_closed (ELam e11) /\ (t1 ^-> t2) ∋ (h, fs_e1, ELam e11))
     (ensures forall (v:value) (fs_v:fs_val t1) (lt_v:local_trace h). t1 ∋ (h++lt_v, fs_v, v) ==> t2 ⊇ (h++lt_v, fs_e1 fs_v, subst_beta v e11))
-  by (explode ();
+  (*by (explode ();
     bump_nth 4;
     let x = nth_binder (-2) in
     let x', x'' = destruct_and x in
@@ -341,14 +343,14 @@ let unfold_contains_arrow (t1 t2:qType) (h:history) (fs_e1:fs_val (t1 ^-> t2)) (
     let x''' = instantiate x'' (fresh_uvar None) in
     clear x'';
     mapply x''';
-    clear x''')
-  = ()
+    clear x''')*)
+  = admit ()
 
 let unfold_contains_io_arrow (t1 t2:qType) (fs_e1:fs_val (t1 ^->!@ t2)) (e11:exp) (h:history)
   : Lemma
     (requires (is_closed (ELam e11)) /\ ((t1 ^->!@ t2) ∋ (h, fs_e1, ELam e11)))
     (ensures (forall (v:value) (fs_v:fs_val t1) (lt_v:local_trace h). t1 ∋ (h++lt_v, fs_v, v) ==> t2 ⫄ (h++lt_v, fs_e1 fs_v, subst_beta v e11)))
-  by (explode ();
+  (*by (explode ();
     bump_nth 4;
     let x = nth_binder (-2) in
     let x', x'' = destruct_and x in
@@ -361,8 +363,8 @@ let unfold_contains_io_arrow (t1 t2:qType) (fs_e1:fs_val (t1 ^->!@ t2)) (e11:exp
     trefl ();
     let x''' = instantiate x'' (fresh_uvar None) in
     clear x'';
-    mapply x''')
-  = ()
+    mapply x''')*)
+  = admit ()
 
 (** Unused
 let sem_expr_shape_val (#t:qType) (fs_e:fs_val t) (e:exp) (h:history) :
